src/HOL/Data_Structures/AVL_Bal2_Set.thy
@@ -1,0 +1,222 @@
+(* Author: Tobias Nipkow *)
+
+section "AVL Tree with Balance Factors (2)"
+
+theory AVL_Bal2_Set
+imports
+  Cmp
+  Isin2
+begin
+
+text \<open>This version passes a flag (\<open>Same\<close>/\<open>Diff\<close>) back up to signal if the height changed.\<close>
+
+datatype bal = Lh | Bal | Rh
+
+type_synonym 'a tree_bal = "('a * bal) tree"
+
+text \<open>Invariant:\<close>
+
+fun avl :: "'a tree_bal \<Rightarrow> bool" where
+"avl Leaf = True" |
+"avl (Node l (a,b) r) =
+  ((case b of
+    Bal \<Rightarrow> height r = height l |
+    Lh \<Rightarrow> height l = height r + 1 |
+    Rh \<Rightarrow> height r = height l + 1)
+  \<and> avl l \<and> avl r)"
+
+
+subsection \<open>Code\<close>
+
+datatype 'a alt = Same 'a | Diff 'a
+
+type_synonym 'a tree_bal2 = "'a tree_bal alt"
+
+fun tree :: "'a alt \<Rightarrow> 'a" where
+"tree(Same t) = t" |
+"tree(Diff t) = t"
+
+fun rot2 where
+"rot2 A a B c C = (case B of
+  (Node B\<^sub>1 (b, bb) B\<^sub>2) \<Rightarrow>
+    let b\<^sub>1 = if bb = Rh then Lh else Bal;
+        b\<^sub>2 = if bb = Lh then Rh else Bal
+    in Node (Node A (a,b\<^sub>1) B\<^sub>1) (b,Bal) (Node B\<^sub>2 (c,b\<^sub>2) C))"
+
+fun balL :: "'a tree_bal2 \<Rightarrow> 'a \<Rightarrow> bal \<Rightarrow> 'a tree_bal \<Rightarrow> 'a tree_bal2" where
+"balL AB' c bc C = (case AB' of
+   Same AB \<Rightarrow> Same (Node AB (c,bc) C) |
+   Diff AB \<Rightarrow> (case bc of
+     Bal \<Rightarrow> Diff (Node AB (c,Lh) C) |
+     Rh \<Rightarrow> Same (Node AB (c,Bal) C) |
+     Lh \<Rightarrow> (case AB of
+       Node A (a,Lh) B \<Rightarrow> Same(Node A (a,Bal) (Node B (c,Bal) C)) |
+       Node A (a,Rh) B \<Rightarrow> Same(rot2 A a B c C))))"
+
+fun balR :: "'a tree_bal \<Rightarrow> 'a \<Rightarrow> bal \<Rightarrow> 'a tree_bal2 \<Rightarrow> 'a tree_bal2" where
+"balR A a ba BC' = (case BC' of
+   Same BC \<Rightarrow> Same (Node A (a,ba) BC) |
+   Diff BC \<Rightarrow> (case ba of
+     Bal \<Rightarrow> Diff (Node A (a,Rh) BC) |
+     Lh \<Rightarrow> Same (Node A (a,Bal) BC) |
+     Rh \<Rightarrow> (case BC of
+       Node B (c,Rh) C \<Rightarrow> Same(Node (Node A (a,Bal) B) (c,Bal) C) |
+       Node B (c,Lh) C \<Rightarrow> Same(rot2 A a B c C))))"
+
+fun ins :: "'a::linorder \<Rightarrow> 'a tree_bal \<Rightarrow> 'a tree_bal2" where
+"ins x Leaf = Diff(Node Leaf (x, Bal) Leaf)" |
+"ins x (Node l (a, b) r) = (case cmp x a of
+   EQ \<Rightarrow> Same(Node l (a, b) r) |
+   LT \<Rightarrow> balL (ins x l) a b r |
+   GT \<Rightarrow> balR l a b (ins x r))"
+
+definition insert :: "'a::linorder \<Rightarrow> 'a tree_bal \<Rightarrow> 'a tree_bal" where
+"insert x t = tree(ins x t)"
+
+fun baldR :: "'a tree_bal \<Rightarrow> 'a \<Rightarrow> bal \<Rightarrow> 'a tree_bal2 \<Rightarrow> 'a tree_bal2" where
+"baldR AB c bc C' = (case C' of
+   Same C \<Rightarrow> Same (Node AB (c,bc) C) |
+   Diff C \<Rightarrow> (case bc of
+     Bal \<Rightarrow> Same (Node AB (c,Lh) C) |
+     Rh \<Rightarrow> Diff (Node AB (c,Bal) C) |
+     Lh \<Rightarrow> (case AB of
+       Node A (a,Lh) B \<Rightarrow> Diff(Node A (a,Bal) (Node B (c,Bal) C)) |
+       Node A (a,Bal) B \<Rightarrow> Same(Node A (a,Rh) (Node B (c,Lh) C)) |
+       Node A (a,Rh) B \<Rightarrow> Diff(rot2 A a B c C))))"
+
+fun baldL :: "'a tree_bal2 \<Rightarrow> 'a \<Rightarrow> bal \<Rightarrow> 'a tree_bal \<Rightarrow> 'a tree_bal2" where
+"baldL A' a ba BC = (case A' of
+   Same A \<Rightarrow> Same (Node A (a,ba) BC) |
+   Diff A \<Rightarrow> (case ba of
+     Bal \<Rightarrow> Same (Node A (a,Rh) BC) |
+     Lh \<Rightarrow> Diff (Node A (a,Bal) BC) |
+     Rh \<Rightarrow> (case BC of
+       Node B (c,Rh) C \<Rightarrow> Diff(Node (Node A (a,Bal) B) (c,Bal) C) |
+       Node B (c,Bal) C \<Rightarrow> Same(Node (Node A (a,Rh) B) (c,Lh) C) |
+       Node B (c,Lh) C \<Rightarrow> Diff(rot2 A a B c C))))"
+
+fun split_max :: "'a tree_bal \<Rightarrow> 'a tree_bal2 * 'a" where
+"split_max (Node l (a, ba) r) =
+  (if r = Leaf then (Diff l,a) else let (r',a') = split_max r in (baldR l a ba r', a'))"
+
+fun del :: "'a::linorder \<Rightarrow> 'a tree_bal \<Rightarrow> 'a tree_bal2" where
+"del _ Leaf = Same Leaf" |
+"del x (Node l (a, ba) r) =
+  (case cmp x a of
+     EQ \<Rightarrow> if l = Leaf then Diff r
+           else let (l', a') = split_max l in baldL l' a' ba r |
+     LT \<Rightarrow> baldL (del x l) a ba r |
+     GT \<Rightarrow> baldR l a ba (del x r))"
+
+definition delete :: "'a::linorder \<Rightarrow> 'a tree_bal \<Rightarrow> 'a tree_bal" where
+"delete x t = tree(del x t)"
+
+lemmas split_max_induct = split_max.induct[case_names Node Leaf]
+
+lemmas splits = if_splits tree.splits alt.splits bal.splits
+
+subsection \<open>Proofs\<close>
+
+subsubsection "Proofs about insertion"
+
+lemma avl_ins_case: "avl t \<Longrightarrow> case ins x t of
+   Same t' \<Rightarrow> avl t' \<and> height t' = height t |
+   Diff t' \<Rightarrow> avl t' \<and> height t' = height t + 1 \<and>
+      (\<forall>l a r. t' = Node l (a,Bal) r \<longrightarrow> a = x \<and> l = Leaf \<and> r = Leaf)"
+apply(induction x t rule: ins.induct)
+apply(auto simp: max_absorb1 split!: splits)
+done
+
+corollary avl_insert: "avl t \<Longrightarrow> avl(insert x t)"
+using avl_ins_case[of t x] by (simp add: insert_def split: splits)
+
+(* The following aux lemma simplifies the inorder_ins proof *)
+
+lemma ins_Diff[simp]: "avl t \<Longrightarrow>
+  ins x t \<noteq> Diff Leaf \<and>
+  (ins x t = Diff (Node l (a,Bal) r) \<longleftrightarrow> t = Leaf \<and> a = x \<and> l=Leaf \<and> r=Leaf) \<and>
+  ins x t \<noteq> Diff (Node l (a,Rh) Leaf) \<and>
+  ins x t \<noteq> Diff (Node Leaf (a,Lh) r)"
+by(drule avl_ins_case[of _ x]) (auto split: splits)
+
+theorem inorder_ins:
+  "\<lbrakk> avl t;  sorted(inorder t) \<rbrakk> \<Longrightarrow> inorder(tree(ins x t)) = ins_list x (inorder t)"
+apply(induction t)
+apply (auto simp: ins_list_simps  split!: splits)
+done
+
+
+subsubsection "Proofs about deletion"
+
+lemma inorder_baldL:
+  "\<lbrakk> ba = Rh \<longrightarrow> r \<noteq> Leaf; avl r \<rbrakk>
+  \<Longrightarrow> inorder (tree(baldL l a ba r)) = inorder (tree l) @ a # inorder r"
+by (auto split: splits)
+
+lemma inorder_baldR:
+  "\<lbrakk> ba = Lh \<longrightarrow> l \<noteq> Leaf; avl l \<rbrakk>
+   \<Longrightarrow> inorder (tree(baldR l a ba r)) = inorder l @ a # inorder (tree r)"
+by (auto split: splits)
+
+lemma avl_split_max:
+  "\<lbrakk> split_max t = (t',a); avl t; t \<noteq> Leaf \<rbrakk> \<Longrightarrow> case t' of
+   Same t' \<Rightarrow> avl t' \<and> height t = height t' |
+   Diff t' \<Rightarrow> avl t' \<and> height t = height t' + 1"
+apply(induction t arbitrary: t' a rule: split_max_induct)
+ apply(fastforce simp: max_absorb1 max_absorb2 split!: splits prod.splits)
+apply simp
+done
+
+lemma avl_del_case: "avl t \<Longrightarrow> case del x t of
+   Same t' \<Rightarrow> avl t' \<and> height t = height t' |
+   Diff t' \<Rightarrow> avl t' \<and> height t = height t' + 1"
+apply(induction x t rule: del.induct)
+ apply(auto simp: max_absorb1 max_absorb2 dest: avl_split_max split!: splits prod.splits)
+done
+
+corollary avl_delete: "avl t \<Longrightarrow> avl(delete x t)"
+using avl_del_case[of t x] by(simp add: delete_def split: splits)
+
+lemma inorder_split_maxD:
+  "\<lbrakk> split_max t = (t',a); t \<noteq> Leaf; avl t \<rbrakk> \<Longrightarrow>
+   inorder (tree t') @ [a] = inorder t"
+apply(induction t arbitrary: t' rule: split_max.induct)
+ apply(fastforce split!: splits prod.splits)
+apply simp
+done
+
+lemma neq_Leaf_if_height_neq_0[simp]: "height t \<noteq> 0 \<Longrightarrow> t \<noteq> Leaf"
+by auto
+
+theorem inorder_del:
+  "\<lbrakk> avl t; sorted(inorder t) \<rbrakk>  \<Longrightarrow> inorder (tree(del x t)) = del_list x (inorder t)"
+apply(induction t rule: tree2_induct)
+apply(auto simp: del_list_simps inorder_baldL inorder_baldR avl_delete inorder_split_maxD
+           simp del: baldR.simps baldL.simps split!: splits prod.splits)
+done
+
+
+subsubsection \<open>Set Implementation\<close>
+
+interpretation S: Set_by_Ordered
+where empty = Leaf and isin = isin
+  and insert = insert
+  and delete = delete
+  and inorder = inorder and inv = avl
+proof (standard, goal_cases)
+  case 1 show ?case by (simp)
+next
+  case 2 thus ?case by(simp add: isin_set_inorder)
+next
+  case 3 thus ?case by(simp add: inorder_ins insert_def)
+next
+  case 4 thus ?case by(simp add: inorder_del delete_def)
+next
+  case 5 thus ?case by (simp)
+next
+  case 6 thus ?case by (simp add: avl_insert)
+next
+  case 7 thus ?case by (simp add: avl_delete)
+qed
+
+end
